Stlc.v
@@ -3,8 +3,6 @@ Require Import Bool.
 Require Import Metalib.Metatheory.
 Require Import List.
 Require Import Ott.ott_list_core.
-(** syntax *)
-Definition expvar : Set := var.
 
 (** For F_p *)
 Require Import Coqprime.elliptic.ZEll.
@@ -15,15 +13,9 @@ From STLCZK Require Import GaloisField.
 
 Module Stlc_Ott(Import PF: GaloisField.GaloisField).
   Import PF.
-      
+  
+  (** syntax *)  
   Definition expvar : Set := var.
-
-  Hint Resolve eq_field: ott_coq_equality.
-  Lemma eq_bool: forall (x y: bool), {x = y} + {x <> y}.
-  Proof.
-    decide equality; auto.
-  Qed.
-  Hint Resolve eq_bool: ott_coq_equality.
 
   Inductive op : Set := 
   | op_add : op
@@ -57,7 +49,8 @@ Module Stlc_Ott(Import PF: GaloisField.GaloisField).
   | tm_pair (e1:exp) (e2:exp)
   | tm_proj_1 (e:exp)
   | tm_proj_2 (e:exp)
-  | tm_cast (e:exp).
+  | tm_to_bool (e:exp)
+  | tm_to_num (e:exp).
 
   Definition typing_env : Set := list (atom*typ).
   Lemma eq_op: forall (x y : op), {x = y} + {x <> y}.
@@ -65,6 +58,12 @@ Module Stlc_Ott(Import PF: GaloisField.GaloisField).
     decide equality; auto with ott_coq_equality arith.
   Defined.
   Hint Resolve eq_op : ott_coq_equality.
+  Hint Resolve eq_field: ott_coq_equality.
+  Lemma eq_bool: forall (x y: bool), {x = y} + {x <> y}.
+  Proof.
+    decide equality; auto.
+  Qed.
+  Hint Resolve eq_bool: ott_coq_equality.
   Lemma eq_typ: forall (x y : typ), {x = y} + {x <> y}.
   Proof.
     decide equality; auto with ott_coq_equality arith.
@@ -100,7 +99,8 @@ Module Stlc_Ott(Import PF: GaloisField.GaloisField).
     | (tm_pair e1 e2) => ((is_value_of_exp e1) && (is_value_of_exp e2))
     | (tm_proj_1 e) => false
     | (tm_proj_2 e) => false
-    | (tm_cast e) => false
+    | (tm_to_bool e) => false
+    | (tm_to_num e) => false
     end.
 
   (** arities *)
@@ -120,7 +120,8 @@ Module Stlc_Ott(Import PF: GaloisField.GaloisField).
     | (tm_pair e1 e2) => tm_pair (open_exp_wrt_exp_rec k e_5 e1) (open_exp_wrt_exp_rec k e_5 e2)
     | (tm_proj_1 e) => tm_proj_1 (open_exp_wrt_exp_rec k e_5 e)
     | (tm_proj_2 e) => tm_proj_2 (open_exp_wrt_exp_rec k e_5 e)
-    | (tm_cast e) => tm_cast (open_exp_wrt_exp_rec k e_5 e)
+    | (tm_to_bool e) => tm_to_bool (open_exp_wrt_exp_rec k e_5 e)
+    | (tm_to_num e) => tm_to_num (open_exp_wrt_exp_rec k e_5 e)
     end.
 
   Definition open_exp_wrt_exp e_5 e__6 := open_exp_wrt_exp_rec 0 e__6 e_5.
@@ -171,10 +172,12 @@ Module Stlc_Ott(Import PF: GaloisField.GaloisField).
   | lc_tm_proj_2 : forall (e:exp),
       (lc_exp e) ->
       (lc_exp (tm_proj_2 e))
-  | lc_tm_cast : forall (e:exp),
+  | lc_tm_to_bool : forall (e:exp),
       (lc_exp e) ->
-      (lc_exp (tm_cast e)).
-
+      (lc_exp (tm_to_bool e))
+  | lc_tm_to_num : forall (e:exp),
+      (lc_exp e) ->
+      (lc_exp (tm_to_num e)).
   (** free variables *)
   Fixpoint fv_exp (e_5:exp) : vars :=
     match e_5 with
@@ -191,7 +194,8 @@ Module Stlc_Ott(Import PF: GaloisField.GaloisField).
     | (tm_pair e1 e2) => (fv_exp e1) \u (fv_exp e2)
     | (tm_proj_1 e) => (fv_exp e)
     | (tm_proj_2 e) => (fv_exp e)
-    | (tm_cast e) => (fv_exp e)
+    | (tm_to_bool e) => (fv_exp e)
+    | (tm_to_num e) => (fv_exp e)
     end.
 
   (** substitutions *)
@@ -210,7 +214,8 @@ Module Stlc_Ott(Import PF: GaloisField.GaloisField).
     | (tm_pair e1 e2) => tm_pair (subst_exp e_5 x5 e1) (subst_exp e_5 x5 e2)
     | (tm_proj_1 e) => tm_proj_1 (subst_exp e_5 x5 e)
     | (tm_proj_2 e) => tm_proj_2 (subst_exp e_5 x5 e)
-    | (tm_cast e) => tm_cast (subst_exp e_5 x5 e)
+    | (tm_to_bool e) => tm_to_bool (subst_exp e_5 x5 e)
+    | (tm_to_num e) => tm_to_num (subst_exp e_5 x5 e)
     end.
 
 
@@ -269,9 +274,12 @@ Module Stlc_Ott(Import PF: GaloisField.GaloisField).
   | typing_proj_2 : forall (G:typing_env) (e:exp) (T2 T1:typ),
       typing G e (ty_prod T1 T2) ->
       typing G (tm_proj_2 e) T2
-  | typing_cast : forall (G:typing_env) (e:exp),
+  | typing_to_num : forall (G:typing_env) (e:exp),
       typing G e ty_bool ->
-      typing G (tm_cast e) ty_field.
+      typing G (tm_to_num e) ty_field
+  | typing_to_bool : forall (G:typing_env) (e:exp),
+      typing G e ty_field ->
+      typing G (tm_to_bool e) ty_bool.
 
   (* defns Jop *)
   Inductive step : exp -> exp -> Prop :=    (* defn step *)
@@ -289,6 +297,11 @@ Module Stlc_Ott(Import PF: GaloisField.GaloisField).
       lc_exp (tm_abs T e1) ->
       lc_exp v2 ->
       step (tm_app  ( (tm_abs T e1) )  v2)  (open_exp_wrt_exp  e1   v2 ) 
+  | step_if_cog : forall (e1 e2 e3 e1':exp),
+      lc_exp e2 ->
+      lc_exp e3 ->
+      step e1 e1' ->
+      step (tm_ifthenelse e1 e2 e3) (tm_ifthenelse e1' e2 e3)
   | step_if_true : forall (e1 e2:exp),
       lc_exp e2 ->
       lc_exp e1 ->
@@ -384,13 +397,22 @@ Module Stlc_Ott(Import PF: GaloisField.GaloisField).
       lc_exp e1 ->
       step e2 e2' ->
       step (tm_pair e1 e2) (tm_pair e1 e2')
-  | step_cast_true : 
-      step (tm_cast (tm_constant (const_bool  true ))) (tm_constant (const_field  1:%p ))
-  | step_cast_false : 
-      step (tm_cast (tm_constant (const_bool  false ))) (tm_constant (const_field  0:%p ))
-  | step_cast_cog : forall (e e':exp),
+  | step_to_num_true : 
+      step (tm_to_num (tm_constant (const_bool  true ))) (tm_constant (const_field  1:%p ))
+  | step_to_num_false : 
+      step (tm_to_num (tm_constant (const_bool  false ))) (tm_constant (const_field  0:%p ))
+  | step_to_num_cog : forall (e e':exp),
       step e e' ->
-      step (tm_cast e) (tm_cast e').
+      step (tm_to_num e) (tm_to_num e')
+  | step_to_bool_true : 
+      step (tm_to_bool (tm_constant (const_field  1:%p ))) (tm_constant (const_bool  true ))
+  | step_to_bool_false : forall (n5:Fp),
+      (const_field n5)  <>  (const_field  1:%p )  ->
+      step (tm_to_bool (tm_constant (const_field n5))) (tm_constant (const_bool  false ))
+  | step_to_bool_cog : forall (e e':exp),
+      step e e' ->
+      step (tm_to_bool e) (tm_to_bool e').
+
 
   (** infrastructure *)
   Hint Constructors typing step lc_exp : core.
@@ -446,7 +468,8 @@ Module Stlc(PF: GaloisField).
   Notation "x == y" := (tm_eq x y) (in custom stlc at level 3,
                                        left associativity).
   Notation "! x " := (tm_not x) (in custom stlc at level 3).
-  Notation "'cast' x" := (tm_cast x) (in custom stlc at level 4).
+  Notation "'to_bool' x" := (tm_to_bool x) (in custom stlc at level 4).
+  Notation "'to_field' x" := (tm_to_num x) (in custom stlc at level 4).
   Notation "'if' x 'then' y 'else' z" :=
     (tm_ifthenelse x y z) (in custom stlc at level 89,
                               x custom stlc at level 99,
@@ -458,7 +481,9 @@ Module Stlc(PF: GaloisField).
                        t1 custom stlc at level 99,
                        t2 custom stlc at level 99,
                    left associativity).
-  Notation "'{' a ',' b '}'" := (tm_pair a b) (in custom stlc at level 5, left associativity).
+  Notation "'{' a ',' b '}'" := (tm_pair a b) (in custom stlc at level 5, right associativity).
   Notation "'fst' a" := (tm_proj_1 a) (in custom stlc at level 5).
   Notation "'snd' a" := (tm_proj_2 a) (in custom stlc at level 5).
 End Stlc.
+
+
